wip

src/Distributions/BernoulliExpNeg/Implementation.dfy
@@ -4,7 +4,9 @@
  *******************************************************************************/
 
 module BernoulliExpNeg.Implementation {
+  import Helper
   import Rationals
+  import Rand
   import Monad
   import Interface
   import Model
@@ -45,28 +47,62 @@ module BernoulliExpNeg.Implementation {
     {
       var k: nat := 0;
       var a := true;
-      ghost var initGamma := gamma;
+      assert GammaLe1LoopInvariant(gamma, old(s), a, k, s) by {
+        reveal GammaLe1LoopInvariant();
+      }
       while a
         decreases *
-        invariant gamma == initGamma
-        invariant Model.GammaLe1Loop(gamma)((a, k))(s) == Model.GammaLe1Loop(gamma)((true, 0))(old(s))
+        invariant 0 <= gamma.numer <= gamma.denom
+        invariant GammaLe1LoopInvariant(gamma, old(s), a, k, s)
       {
         ghost var prevK: nat := k;
         ghost var prevA := a;
         ghost var prevS := s;
         k := k + 1;
-        assume gamma.numer < k * gamma.denom;
+        Helper.MulMonotonic(1, gamma.denom, k, gamma.denom);
         a := BernoulliSample(Rationals.Rational(gamma.numer, k * gamma.denom));
-        assert ((a, k), s) == Model.GammaLe1LoopIter(gamma)((prevA, prevK))(prevS) by {
-          Model.GammaLe1LoopIterProperty(gamma, prevA, prevK, prevS, a, k, s);
-        }
-        assert Model.GammaLe1Loop(gamma)((prevA, prevK))(prevS) == Model.GammaLe1Loop(gamma)((a, k))(s) by {
-          Model.GammaLe1LoopUnroll(gamma, (prevA, prevK), prevS);
-        }
+        Model.GammaLe1LoopIterProperty(gamma, prevA, prevK, prevS, a, k, s);
+        EnsureLoopInvariant(gamma, old(s), prevK, prevS, a, k, s);
       }
       c := k % 2 == 1;
-      assume {:axiom} Monad.Result(c, s) == Model.SampleGammaLe1(gamma)(old(s)); // add later
+      EnsurePostCondition(gamma, old(s), k, s, c);
     }
 
+    opaque ghost predicate GammaLe1LoopInvariant(gamma: Rationals.Rational, oldS: Rand.Bitstream, a: bool, k: nat, s: Rand.Bitstream)
+      requires 0 <= gamma.numer <= gamma.denom
+    {
+      Model.GammaLe1Loop(gamma)((true, 0))(oldS) == Model.GammaLe1Loop(gamma)((a, k))(s)
+    }
+
+    lemma EnsureLoopInvariant(gamma: Rationals.Rational, oldS: Rand.Bitstream, k: nat, s: Rand.Bitstream, a': bool, k': nat, s': Rand.Bitstream)
+      requires 0 <= gamma.numer <= gamma.denom
+      requires inv: GammaLe1LoopInvariant(gamma, oldS, true, k, s)
+      requires iter: Monad.Result((a', k'), s') == Model.GammaLe1LoopIter(gamma)((true, k))(s)
+      ensures GammaLe1LoopInvariant(gamma, oldS, a', k', s')
+    {
+      calc {
+        Model.GammaLe1Loop(gamma)((true, 0))(oldS);
+        { reveal GammaLe1LoopInvariant(); reveal inv; }
+        Model.GammaLe1Loop(gamma)((true, k))(s);
+        { reveal iter; Model.GammaLe1LoopUnroll(gamma, (true, k), s); }
+        Model.GammaLe1Loop(gamma)((a', k'))(s');
+      }
+      reveal GammaLe1LoopInvariant();
+    }
+
+    lemma EnsurePostCondition(gamma: Rationals.Rational, oldS: Rand.Bitstream, k: nat, s: Rand.Bitstream, c: bool)
+      requires 0 <= gamma.numer <= gamma.denom
+      requires GammaLe1LoopInvariant(gamma, oldS, false, k, s)
+      requires c <==> (k % 2 == 1)
+      ensures Monad.Result(c, s) == Model.SampleGammaLe1(gamma)(oldS)
+    {
+      calc {
+        Model.GammaLe1Loop(gamma)((true, 0))(oldS);
+        { reveal GammaLe1LoopInvariant(); }
+        Model.GammaLe1Loop(gamma)((false, k))(s);
+        { reveal Model.GammaLe1Loop(); }
+        Monad.Result((false, k), s);
+      }
+    }
   }
 }
