src/Distributions/BernoulliExpNeg/Model.dfy
@@ -67,7 +67,7 @@ module BernoulliExpNeg.Model {
     )
   }
 
-  ghost function GammaLe1Loop(gamma: Rationals.Rational): ((bool, nat)) -> Monad.Hurd<(bool, nat)>
+  opaque ghost function GammaLe1Loop(gamma: Rationals.Rational): ((bool, nat)) -> Monad.Hurd<(bool, nat)>
     requires 0 <= gamma.numer <= gamma.denom
   {
     (ak: (bool, nat)) =>
@@ -93,15 +93,21 @@ module BernoulliExpNeg.Model {
       res
   }
 
+  lemma SampleGammaLe1Property(gamma: Rationals.Rational, k: nat, s: Rand.Bitstream)
+    requires 0 <= gamma.numer <= gamma.denom
+    requires Monad.Result((false, k), s) == GammaLe1Loop(gamma)((true, 0))(s)
+    ensures Monad.Result(k % 2 == 1, s) == SampleGammaLe1(gamma)(s)
+  {}
+
   lemma {:vcs_split_on_every_assert} GammaLe1LoopIterProperty(gamma: Rationals.Rational, a: bool, k: nat, s: Rand.Bitstream, a': bool, k': nat, s': Rand.Bitstream)
     requires 0 <= gamma.numer <= gamma.denom
     requires k' == k + 1
-    requires (a' , s') == Bernoulli.Model.Sample(gamma.numer, k' * gamma.denom)(s)
-    ensures ((a', k'), s') == GammaLe1LoopIter(gamma)((a,k))(s)
+    requires Monad.Result(a' , s') == Bernoulli.Model.Sample(gamma.numer, k' * gamma.denom)(s)
+    ensures Monad.Result((a', k'), s') == GammaLe1LoopIter(gamma)((a,k))(s)
   {
-    var (a, s') := Bernoulli.Model.Sample(gamma.numer, k' * gamma.denom)(s);
-    assert GammaLe1LoopIter(gamma)((a, k))(s) == ((a', k'), s');
-    assert Monad.Bind(Bernoulli.Model.Sample(gamma.numer, k' * gamma.denom), a => Monad.Return((a, k')))(s) == ((a, k'), s');
+    var Result(a, s') := Bernoulli.Model.Sample(gamma.numer, k' * gamma.denom)(s);
+    assert GammaLe1LoopIter(gamma)((a, k))(s) == Monad.Result((a', k'), s');
+    assert Monad.Bind(Bernoulli.Model.Sample(gamma.numer, k' * gamma.denom), a => Monad.Return((a, k')))(s) == Monad.Result((a, k'), s');
   }
 
   lemma {:axiom} GammaLe1LoopTerminatesAlmostSurely(gamma: Rationals.Rational)
